Updates.

FOL/Fresh.lean
@@ -6,18 +6,18 @@ set_option autoImplicit false
 
 
 /--
-  finset_var_name_max_len xs := The length of the longest variable name in the finite set of variable names xs or 0 if the set is empty.
+  finset_string_max_len xs := The length of the longest variable name in the finite set of variable names xs or 0 if the set is empty.
 -/
-def finset_var_name_max_len :
+def finset_string_max_len :
   Finset VarName → ℕ :=
   Finset.fold (fun (m n : ℕ) => max m n) 0 (String.length ∘ VarName.toString)
 
 
-lemma finset_var_name_max_len_mem
+lemma finset_string_max_len_mem
   (x : VarName)
   (xs : Finset VarName)
   (h1 : x ∈ xs) :
-  x.length <= finset_var_name_max_len xs :=
+  x.length <= finset_string_max_len xs :=
   by
   induction xs using Finset.induction_on
   case empty =>
@@ -28,12 +28,12 @@ lemma finset_var_name_max_len_mem
     cases h1
     case inl c1 =>
       subst c1
-      simp only [finset_var_name_max_len]
+      simp only [finset_string_max_len]
       simp
     case inr c1 =>
-      simp only [finset_var_name_max_len] at ih
+      simp only [finset_string_max_len] at ih
 
-      simp only [finset_var_name_max_len]
+      simp only [finset_string_max_len]
       simp
       right
       exact ih c1
@@ -49,14 +49,14 @@ def fresh
   VarName :=
   if h : x ∈ xs
   then
-    have : finset_var_name_max_len xs - String.length x.toString < finset_var_name_max_len xs + 1 - String.length x.toString :=
+    have : finset_string_max_len xs - String.length x.toString < finset_string_max_len xs + 1 - String.length x.toString :=
       by
-      obtain s1 := finset_var_name_max_len_mem x xs h
+      obtain s1 := finset_string_max_len_mem x xs h
       simp only [tsub_lt_tsub_iff_right s1]
       simp
   fresh (VarName.mk (x.toString ++ c.toString)) c xs
   else x
-  termination_by finset_var_name_max_len xs + 1 - x.length
+  termination_by finset_string_max_len xs + 1 - x.length
 
 
 lemma fresh_not_mem
@@ -66,9 +66,9 @@ lemma fresh_not_mem
   fresh x c xs ∉ xs :=
   if h : x ∈ xs
   then
-  have : finset_var_name_max_len xs - String.length x.toString < finset_var_name_max_len xs + 1 - String.length x.toString :=
+  have : finset_string_max_len xs - String.length x.toString < finset_string_max_len xs + 1 - String.length x.toString :=
     by
-    obtain s1 := finset_var_name_max_len_mem x xs h
+    obtain s1 := finset_string_max_len_mem x xs h
     simp only [tsub_lt_tsub_iff_right s1]
     simp
   by
@@ -81,7 +81,7 @@ lemma fresh_not_mem
     simp
     simp [if_neg h]
     exact h
-  termination_by finset_var_name_max_len xs + 1 - x.length
+  termination_by finset_string_max_len xs + 1 - x.length
 
 
 #lint
